finish porting heapLang related theorem

IrisITree/IrisITree/Effects/Step.lean
@@ -1,9 +1,137 @@
 module
 
+import Iris.ProofMode
+public import IrisITree.Core.Wpi
+public import ITree.Effects.Step
+public import Iris.Instances.Lib.FUpd
+
 @[expose] public section
 
--- Step events. The main application of this event type is for doing
--- termination insensitive reasoning in spite of our [WPi] being defined as a
--- least fixpoint (and thus being termination sensitive "by default").
-
 namespace IrisITree.Effects
+
+open Iris Iris.BI ITree ITree.Effects IrisITree.Core
+
+section handler
+
+variable {PROP : Type _} [BI PROP]
+
+/-- A logical modality used to interpret operational `step` events. -/
+class StepMod (PROP : Type _) [BI PROP] where
+  apply : PROP → PROP
+  mono (P Q : PROP) : ⊢@{PROP} (P -∗ Q) -∗ apply P -∗ apply Q
+
+instance : CoeFun (StepMod PROP) (λ _ => PROP → PROP) where
+  coe m := @StepMod.apply PROP _ m
+
+namespace StepMod
+
+theorem map (m : StepMod PROP) (P Q : PROP) :
+    ⊢@{PROP} m P -∗ (P -∗ Q) -∗ m Q := by
+  iintro HP Hwand
+  iapply (@StepMod.mono PROP _ m P Q) $$ Hwand HP
+
+/-- Interpret a step without adding a logical modality. -/
+@[reducible] def ident : StepMod PROP where
+  apply P := P
+  mono _ _ := by
+    iintro Hwand HP
+    iapply Hwand $$ [$]
+
+/-- Interpret a step as one logical later. -/
+@[reducible] def later : StepMod PROP where
+  apply P := iprop(▷ P)
+  mono _ _ := by
+    iintro Hwand HP
+    inext; iapply Hwand $$ [$]
+
+theorem wand (m : StepMod PROP) (P Q : PROP) :
+    ⊢@{PROP} m iprop(P -∗ Q) -∗ P -∗ m Q := by
+  iintro Hwand HP
+  iapply m.map $$ Hwand
+  iintro HPQ
+  iapply HPQ $$ HP
+
+end StepMod
+
+/-- Interpret an operational step using `m`. -/
+def stepH (m : StepMod PROP) : IHandler PROP stepE where
+  ihandle := λ _ Φ _ => m (Φ ⟨⟩)
+  ihandle_mono := by
+    iintro %_ %Φ %Φ' %_ %_ HΦwand _ HΦ
+    ispecialize HΦwand $$ %⟨⟩
+    iapply m.map $$ HΦ HΦwand
+
+instance stepH_sequential (m : StepMod PROP) : Sequential (stepH m) := by
+  constructor
+  iintro %_ %_ %_ H
+  simp only [stepH]
+  iexact H
+
+/-- An identity step interpretation implies a later step interpretation. -/
+instance stepH_ident_later :
+    WandH (stepH .ident (PROP := PROP)) (stepH .later) := by
+  constructor
+  intro _ _ _
+  exact entails_wand later_intro
+
+end handler
+
+section wpi_rules
+
+variable {PROP : Type _} [BI PROP] [BIFUpdate PROP]
+  {E : Effect} {H : IHandler PROP E}
+  {m : StepMod PROP}
+  [sub : stepE -< E] [Hin : InH (stepH m) H]
+
+theorem wpi_step M (Φ : PUnit → PROP) :
+    m iprop(|={M}=> Φ ⟨⟩) -∗
+    WPi step @> H; M {{ Φ }} := by
+  change m iprop(|={M}=> Φ ⟨⟩) -∗
+    WPi (@Effect.trigger stepE E sub ⟨⟩) @> H; M {{ Φ }}
+  iintro HΦ; iapply wpi_trigger
+  iapply fupd_mask_intro (by simp)
+  iintro Hclose; simp only [stepH]
+  iapply m.map $$ HΦ
+  iintro HΦ; imod Hclose; imod HΦ
+  imodintro; iframe
+
+end wpi_rules
+
+section exec
+
+open ITree.Exec
+
+variable {GF : BundledGFunctors} [InvGS GF]
+
+/-- Executing an identity-interpreted step requires no later credits. -/
+instance stepEH_ident_adequate :
+    SEHandlerAdequate (stepH (.ident (PROP := IProp GF))) (stepEH (λ _ => 0)) where
+  inv _ := iprop(True)
+  adequate := by
+    intro i s C Φ₁ Φ₂ Hhandle
+    simp only [stepH, stepEH] at *
+    simp only [Nat.zero_le, true_and, Nat.sub_zero] at Hhandle
+    iintro HΦ _ !>
+    iexists ⟨⟩, (ULift.up (s.1.down + 1), ULift.up s.2.down)
+    iframe; itrivial
+
+/-- Executing a later-interpreted step consumes one later credit. -/
+instance stepEH_later_adequate :
+    SEHandlerAdequate (stepH (.later (PROP := IProp GF))) (stepEH (λ _ => 1)) where
+  inv s := £ s.2.down
+  adequate := by
+    intro i s C Φ₁ Φ₂ Hhandle
+    simp only [stepH, stepEH] at *
+    obtain ⟨Hcredit, HC⟩ := Hhandle
+    iintro HΦ Hlc
+    ihave Hparts : £ 1 ∗ £ (s.2.down - 1) $$ [Hlc]
+    · iapply lc_split.mp
+      rw [Nat.add_sub_of_le Hcredit]
+      iexact Hlc
+    icases Hparts with ⟨Hone, Hrest⟩
+    imod lc_fupd_elim_later $$ Hone HΦ with HΦ
+    imodintro
+    iexists ⟨⟩, (ULift.up (s.1.down + 1), ULift.up (s.2.down - 1))
+    iframe; itrivial
+
+end exec
