IrisITree/IrisITree/HeapLang/ProgramLogic.lean
@@ -10,64 +10,463 @@ public import Iris.Instances.Lib.FUpd
 @[expose] public section
 namespace IrisITree.HeapLang
 
-open Iris IrisITree.Core Iris.HeapLang IrisITree.Effects
+open Iris IrisITree.Core Iris.HeapLang IrisITree.Effects ITree ITree.Effects
 
-section wp
-variable {GF} [InvGS GF] {m : Unit}
+class heaplangHGpreS (GF : BundledGFunctors) where
+  heaplangH_heapHG : heapHGpreS GF Loc Val
 
-def heaplangH : IHandler (IProp GF) heaplangE := concH ⊕ₕ (by sorry) ⊕ₕ failH ⊕ₕ demonicH Loc ⊕ₕ by sorry
+attribute [reducible, instance] heaplangHGpreS.heaplangH_heapHG
 
-instance wp_heaplang : Wp (IProp GF) Exp Val Unit where
-  wp _ E e Φ := WPi e.denote @> heaplangH; E {{ Φ }}
+class heaplangHGS (GF : BundledGFunctors) where
+  heaplangH_heapHGS : heapHGS GF Loc Val
 
-theorem wp_unfold (e : Exp) (Φ : Val → IProp GF) :
-  WP e @ m ; E {{ Φ }} = WPi e.denote @> heaplangH; E {{ Φ }} := rfl
+attribute [reducible, instance] heaplangHGS.heaplangH_heapHGS
 
--- TODO
-/-
-  Lemma wp_bind m K e Φ :
-    WP e @ m; ⊤ {{ v,
-      WP fill K (Val v) @ m; ⊤ {{ Φ }}
-    }} -∗
-    WP fill K e @ m; ⊤ {{ Φ }}.
--/
+instance lawfulLoc_heaplang : LawfulLoc Loc where
+  decEq := inferInstance
+  add_zero l := by ext; simp
+  add_nat_inj l := by
+    intro i j Hij
+    have Hn := congrArg Loc.n Hij
+    simp at Hn
+    omega
+  add_pos_nle := by
+    intro l m
+    simp [compare, compareOfLessAndEq, Ordering.isLE]
+    grind
 
-theorem wp_wand E (e : Exp) (Φ Ψ : Val → IProp GF) :
-  WP e @ m ; E {{ Φ }} -∗
-  (∀ v, Φ v -∗ Ψ v) -∗
-  WP e @ m ; E {{ Ψ }} := by
-    simp only [wp_unfold]
-    apply wpi_wand
+section handler
+
+variable {GF} [InvGS GF] [heaplangHGS GF]
+
+def heaplangH (m : StepMod (IProp GF)) : IHandler (IProp GF) heaplangE :=
+  concH ⊕ₕ heapH ⊕ₕ failH ⊕ₕ demonicH Loc ⊕ₕ stepH m
+
+instance inH_conc_heaplang (m : StepMod (IProp GF)) :
+    InH concH (heaplangH m) := by
+  unfold heaplangH
+  infer_instance
+
+instance inH_heap_heaplang (m : StepMod (IProp GF)) :
+    InH (heapH (Loc := Loc) (Val := Val)) (heaplangH m) := by
+  unfold heaplangH
+  infer_instance
+
+instance inH_fail_heaplang (m : StepMod (IProp GF)) :
+    InH failH (heaplangH m) := by
+  unfold heaplangH
+  infer_instance
+
+instance inH_demonic_heaplang (m : StepMod (IProp GF)) :
+    InH (demonicH Loc) (heaplangH m) := by
+  unfold heaplangH
+  infer_instance
+
+instance inH_step_heaplang (m : StepMod (IProp GF)) :
+    InH (stepH m) (heaplangH m) := by
+  unfold heaplangH
+  infer_instance
+
+instance wandH_heaplang_ident_later :
+    WandH (heaplangH (.ident (PROP := IProp GF))) (heaplangH .later) := by
+  unfold heaplangH
+  infer_instance
+
+instance wp_heaplang : Wp (IProp GF) Exp Val (StepMod (IProp GF)) where
+  wp m M e Φ := WPi e.denote @> heaplangH m; M {{ Φ }}
+
+end handler
+
+section wpi_rules
+
+variable {GF} [InvGS GF] [heaplangHGS GF]
+  {m : StepMod (IProp GF)}
+
+theorem wpi_step_pure E (v : Val) (Φ : Val → IProp GF) :
+    m (Φ v) -∗
+    WPi (do
+      step
+      pure v) @> heaplangH m; E {{ Φ }} := by
+  iintro HΦ
+  iapply wpi_bind
+  iapply wpi_step
+  iapply m.map $$ HΦ
+  iintro HΦ
+  imodintro
+  iapply wpi_pure $$ HΦ
+
+theorem wpi_yieldIfNotVal (e : Exp) (Φ : Unit → IProp GF) :
+    Φ () -∗
+    WPi e.yieldIfNotVal @> heaplangH m; ⊤ {{ Φ }} := by
+  cases e <;> simp only [Exp.yieldIfNotVal]
+  · iintro HΦ; iapply wpi_pure $$ [$]
+  all_goals
+    iintro HΦ; iapply wpi_yield $$ [$]
+
+theorem wpi_cont (e : Exp) (Φ : Val → IProp GF) :
+    m (WP e @ m ; ⊤ {{ Φ }}) -∗
+    WPi (do
+      step
+      e.yieldIfNotVal
+      e.denote) @> heaplangH m; ⊤ {{ Φ }} := by
+  iintro Hwp; iapply wpi_bind
+  iapply wpi_step
+  iapply m.map $$ Hwp
+  iintro Hwp !>; iapply wpi_bind
+  iapply wpi_yieldIfNotVal; iframe
+
+end wpi_rules
+
+section wp_rules
+
+variable {GF} [InvGS GF] [heaplangHGS GF]
+  {m : StepMod (IProp GF)}
+
+theorem wp_unfold {M : CoPset} (e : Exp) (Φ : Val → IProp GF) :
+  WP e @ m; M {{ Φ }} = WPi e.denote @> heaplangH m; M {{ Φ }} := rfl
+
+/-- The identity (total) WP implies the later (partial) WP. -/
+theorem wp_later_weaken {M : CoPset} (e : Exp) (Φ : Val → IProp GF) :
+    WP e @ (StepMod.ident (PROP := IProp GF)); M {{ Φ }} -∗
+    WP e @ (StepMod.later (PROP := IProp GF)); M {{ Φ }} := by
+  simp only [wp_unfold]
+  iintro Hwp
+  iapply (wpi_wandH
+    (H1 := heaplangH (StepMod.ident (PROP := IProp GF)))
+    (H2 := heaplangH (StepMod.later (PROP := IProp GF))))
+  iexact Hwp
+
+-- theorem wp_bind (K : List ECtxItem) (e : Exp) (Φ : Val → IProp GF) :
+--     WP e @ m; ⊤ {{ v,
+--       WP (ProgramLogic.fill K (Exp.ofVal (Expr := Exp) v)) @ m; ⊤ {{ Φ }}
+--     }} -∗
+--     WP (ProgramLogic.fill K e) @ m; ⊤ {{ Φ }} := by
+--   sorry
+
+theorem wp_wand {M : CoPset} (e : Exp) (Φ Ψ : Val → IProp GF) :
+    WP e @ m ; M {{ Φ }} -∗
+    (∀ v, Φ v -∗ Ψ v) -∗
+    WP e @ m ; M {{ Ψ }} := by
+  simp only [wp_unfold]
+  apply wpi_wand
+
+theorem wp_frame_l {M : CoPset} (e : Exp) (Φ : Val → IProp GF) :
+    P ∗ WP e @ m; M {{ Φ }} -∗ WP e @ m; M {{v , P ∗ Φ v}} := by
+  iintro ⟨HP, Hwp⟩
+  iapply wp_wand $$ Hwp [HP]
+  iintro %_ _; iframe
 
 theorem wp_atomic E1 E2 (e : Exp) (Φ : Val → IProp GF) :
-  (|={E1,E2}=> WP e @ m ; E2 {{ v, |={E2,E1}=> Φ v }}) ⊢
-  WP e @ m ; E1 {{ Φ }} := by
-    simp only [wp_unfold]
-    iintro > >Hwp
-    iapply wpi_fupd_empty
-    ihave Hwp := wpi_fupd_empty $$ Hwp
-    iapply wpi_wand $$ Hwp
-    iintro %_ > > $
+    (|={E1,E2}=> WP e @ m ; E2 {{ v, |={E2,E1}=> Φ v }}) ⊢ WP e @ m ; E1 {{ Φ }} := by
+  simp only [wp_unfold]
+  iintro > >Hwp
+  iapply wpi_fupd_empty
+  ihave Hwp := wpi_fupd_empty $$ Hwp
+  iapply wpi_wand $$ Hwp
+  iintro %_ > > $
 
-theorem fupd_wp E (e : Exp) (Φ : Val → IProp GF) :
-  (|={E}=> WP e @ m ; E {{ v, Φ v }}) ⊢ WP e @ m ; E {{ Φ }} := by
-    simp only [wp_unfold]
-    iapply (fupd_wpi _).2
+theorem fupd_wp {M : CoPset} (e : Exp) (Φ : Val → IProp GF) :
+    (|={M}=> WP e @ m ; M {{ v, Φ v }}) ⊢ WP e @ m ; M {{ Φ }} := by
+  simp only [wp_unfold]
+  iapply (fupd_wpi _).2
 
-theorem wp_fupd E (e : Exp) (Φ : Val → IProp GF) :
-  (WP e @ m ; E {{ v, |={E}=> Φ v }}) ⊢ WP e @ m ; E {{ Φ }} := by
-    simp only [wp_unfold]
-    iapply (wpi_fupd _).2
+theorem wp_fupd {M : CoPset} (e : Exp) (Φ : Val → IProp GF) :
+    (WP e @ m ; M {{ v, |={M}=> Φ v }}) ⊢ WP e @ m ; M {{ Φ }} := by
+  simp only [wp_unfold]
+  iapply (wpi_fupd _).2
 
--- # Proof rules for pure operations
-
-theorem wp_val E (v : Val) (Φ : Val → IProp GF) :
+theorem wp_val {M : CoPset} (v : Val) (Φ : Val → IProp GF) :
     Φ v -∗
-    WP hl(v(&v)) @ m ; E {{ Φ }} := by
-  sorry
-  -- simp only [wp_unfold, Exp.denote]
-  -- iapply wpi_pure
+    WP hl(v(&v)) @ m ; M {{ Φ }} := by
+  iintro HΦ
+  simp only [wp_unfold]
+  rw [← val_to_ofVal, Exp.denote.eq_1]
+  iapply wpi_pure $$ [$]
 
--- TODO...
+theorem wp_unop {M : CoPset} (op : UnOp) (v v' : Val) (Φ : Val → IProp GF) :
+    ⌜op.denote v = pure v'⌝ -∗
+    m (Φ v') -∗
+    WP (Exp.unop op (Exp.val v)) @ m ; M {{ Φ }} := by
+  iintro %Hop HΦ
+  simp only [wp_unfold, Exp.denote.eq_5, Exp.isVal, ↓reduceIte,
+    Exp.denote.eq_1, LawfulMonad.pure_bind]
+  rw [Hop]
+  simp only [LawfulMonad.pure_bind]
+  iapply wpi_step_pure $$ [$]
 
-end wp
+theorem wp_binop {M : CoPset} (op : BinOp) (v₁ v₂ v' : Val) (Φ : Val → IProp GF) :
+    ⌜op.denote v₁ v₂ = pure v'⌝ -∗
+    m (Φ v') -∗
+    WP (Exp.binop op (Exp.val v₁) (Exp.val v₂)) @ m ; M {{ Φ }} := by
+  iintro % Hop HΦ
+  simp only [wp_unfold, Exp.denote.eq_6, Exp.isVal, ↓reduceIte,
+    Exp.denote.eq_1, LawfulMonad.pure_bind]
+  rw [Hop]
+  simp only [LawfulMonad.pure_bind]
+  iapply wpi_step_pure $$ [$]
+
+theorem wp_if_true (e₁ e₂ : Exp) (Φ : Val → IProp GF) :
+    m (WP e₁ @ m ; ⊤ {{ Φ }}) -∗
+    WP (Exp.if (Exp.val (Val.lit (BaseLit.bool true))) e₁ e₂) @ m ; ⊤ {{ Φ }} := by
+  iintro Hwp
+  simp only [wp_unfold, Exp.denote.eq_7, Exp.isVal, ↓reduceIte]
+  iapply wpi_bind; iapply wp_val
+  iapply wpi_bind; simp only [Val.bool!]
+  iapply wpi_pure; simp only [↓reduceIte]
+  iapply wpi_cont $$ [$]
+
+theorem wp_if_false (e₁ e₂ : Exp) (Φ : Val → IProp GF) :
+    m (WP e₂ @ m ; ⊤ {{ Φ }}) -∗
+    WP (Exp.if (Exp.val (Val.lit (BaseLit.bool false))) e₁ e₂) @ m ; ⊤ {{ Φ }} := by
+  iintro Hwp
+  simp only [wp_unfold, Exp.denote.eq_7, Exp.isVal, ↓reduceIte]
+  iapply wpi_bind; iapply wp_val
+  iapply wpi_bind; simp only [Val.bool!]
+  iapply wpi_pure; simp only [Bool.false_eq_true, ↓reduceIte]
+  iapply wpi_cont $$ [$]
+
+theorem wp_app (f x : Binder) (v : Val) (e : Exp) (Φ : Val → IProp GF) :
+    m (WP ((e.subst f (.rec_ f x e)).subst x v) @ m ; ⊤ {{ Φ }}) -∗
+    WP (Exp.app (Exp.val (Val.rec_ f x e)) (Exp.val v)) @ m ; ⊤ {{ Φ }} := by
+  iintro Hwp
+  simp only [wp_unfold, Exp.denote.eq_4, Exp.isVal, ↓reduceIte,
+    Exp.denote.eq_1, LawfulMonad.pure_bind, Val.rec!]
+  iapply wpi_cont $$ [$]
+
+theorem wp_rec {M : CoPset} (f x : Binder) (e : Exp) (Φ : Val → IProp GF) :
+    m (Φ (.rec_ f x e)) -∗
+    WP (Exp.rec_ f x e) @ m ; M {{ Φ }} := by
+  iintro HΦ
+  simp only [wp_unfold, Exp.denote.eq_3]
+  iapply wpi_step_pure $$ [$]
+
+theorem wp_pair {M : CoPset} (v₁ v₂ : Val) (Φ : Val → IProp GF) :
+    m (Φ (.pair v₁ v₂)) -∗
+    WP (Exp.pair (.val v₁) (.val v₂)) @ m ; M {{ Φ }} := by
+  iintro HΦ
+  simp only [wp_unfold, Exp.denote.eq_8, Exp.isVal, ↓reduceIte,
+    Exp.denote.eq_1, LawfulMonad.pure_bind]
+  iapply wpi_step_pure $$ [$]
+
+theorem wp_fst {M : CoPset} (v₁ v₂ : Val) (Φ : Val → IProp GF) :
+    m (Φ v₁) -∗
+    WP (Exp.fst (.val (.pair v₁ v₂))) @ m ; M {{ Φ }} := by
+  iintro HΦ
+  simp only [wp_unfold, Exp.denote.eq_9, Exp.isVal, ↓reduceIte]
+  iapply wpi_bind; iapply wp_val
+  iapply wpi_bind; simp only [Val.pair!]
+  iapply wpi_pure
+  iapply wpi_step_pure $$ [$]
+
+theorem wp_snd {M : CoPset} (v₁ v₂ : Val) (Φ : Val → IProp GF) :
+    m (Φ v₂) -∗
+    WP (Exp.snd (.val (.pair v₁ v₂))) @ m ; M {{ Φ }} := by
+  iintro HΦ
+  simp only [wp_unfold, Exp.denote.eq_10, Exp.isVal, ↓reduceIte]
+  iapply wpi_bind; iapply wp_val
+  iapply wpi_bind; simp only [Val.pair!]
+  iapply wpi_pure
+  iapply wpi_step_pure $$ [$]
+
+theorem wp_injL {M : CoPset} (v : Val) (Φ : Val → IProp GF) :
+    m (Φ (.injL v)) -∗
+    WP (Exp.injL (.val v)) @ m ; M {{ Φ }} := by
+  iintro HΦ
+  simp only [wp_unfold, Exp.denote.eq_11, Exp.isVal, ↓reduceIte]
+  iapply wpi_bind; iapply wp_val
+  iapply wpi_step_pure $$ [$]
+
+theorem wp_injR {M : CoPset} (v : Val) (Φ : Val → IProp GF) :
+    m (Φ (.injR v)) -∗
+    WP (Exp.injR (.val v)) @ m ; M {{ Φ }} := by
+  iintro HΦ
+  simp only [wp_unfold, Exp.denote.eq_12, Exp.isVal, ↓reduceIte]
+  iapply wpi_bind; iapply wp_val
+  iapply wpi_step_pure $$ [$]
+
+theorem wp_caseL (v : Val) (e₁ e₂ : Exp) (Φ : Val → IProp GF) :
+    m (WP (Exp.app e₁ (Exp.val v)) @ m ; ⊤ {{ Φ }}) -∗
+    WP (Exp.case (Exp.val (Val.injL v)) e₁ e₂) @ m ; ⊤ {{ Φ }} := by
+  iintro Hwp
+  simp only [wp_unfold, Exp.denote.eq_13, Exp.isVal, ↓reduceIte]
+  iapply wpi_bind; iapply wp_val
+  iapply wpi_cont $$ [$]
+
+theorem wp_caseR (v : Val) (e₁ e₂ : Exp) (Φ : Val → IProp GF) :
+    m (WP (Exp.app e₂ (Exp.val v)) @ m ; ⊤ {{ Φ }}) -∗
+    WP (Exp.case (Exp.val (Val.injR v)) e₁ e₂) @ m ; ⊤ {{ Φ }} := by
+  iintro Hwp
+  simp only [wp_unfold, Exp.denote.eq_13, Exp.isVal, ↓reduceIte]
+  iapply wpi_bind; iapply wp_val
+  iapply wpi_cont $$ [$]
+
+theorem wp_fork (e : Exp) (Φ : Val → IProp GF) :
+    m (Φ (.lit .unit)) -∗
+    WP e @ m; ⊤ {{ v, ⌜v = .lit .unit⌝ }} -∗
+    WP (Exp.fork e) @ m; ⊤ {{ Φ }} := by
+  iintro HΦ Hwp
+  simp only [wp_unfold, Exp.denote.eq_21, Exp.isVal]
+  iapply wpi_bind; iapply wpi_fork $$ [HΦ]
+  · iapply wpi_step_pure $$ [$]
+  · iapply wpi_bind;
+    cases e <;> simp only [↓reduceIte, ConcE.yieldAfter, Bool.false_eq_true]
+    · iapply wpi_wand $$ Hwp;
+      iintro %_ _; iapply wpi_pure; itrivial
+    all_goals
+      iapply wpi_bind; iapply wpi_wand $$ Hwp
+      iintro %_ _; iapply wpi_bind; iapply wpi_yield
+      iapply wpi_pure; iapply wpi_pure; itrivial
+
+section heap_rules
+
+theorem wp_allocN {M : CoPset} (n : Int) (v : Val) (Φ : Val → IProp GF) :
+    0 < n →
+    ↑(heapH_inv_name (GF := GF) (Loc := Loc) (Val := Val)) ⊆ M →
+    m iprop(∀ l : Loc,
+      ([∗list] i ∈ List.range n.toNat, (l + Int.ofNat i) ↦ v) -∗
+      Φ (.lit (.loc l))) -∗
+    WP (Exp.allocN (.val (.lit (.int n))) (.val v)) @ m; M {{ Φ }} := by
+  iintro %Hpos %Hmask HΦ
+  simp only [wp_unfold, Exp.denote.eq_14, Exp.isVal, ↓reduceIte]
+  iapply wpi_bind; iapply wp_val
+  iapply wpi_bind; iapply wp_val
+  iapply wpi_bind; simp only [Val.int!];
+  iapply wpi_pure; simp only [Int.not_le.mpr Hpos, ↓reduceIte]
+  iapply wpi_bind; iapply wpi_allocN _ _ _ _ Hmask
+  iintro %l Hpts; iapply wpi_step_pure
+  iapply m.map $$ HΦ
+  iintro HΦ; ispecialize HΦ $$ %l
+  iapply HΦ $$ Hpts
+
+theorem wp_alloc {M : CoPset} (v : Val) (Φ : Val → IProp GF) :
+    ↑(heapH_inv_name (GF := GF) (Loc := Loc) (Val := Val)) ⊆ M →
+    m iprop(∀ l, l ↦ v -∗ Φ (.lit (.loc l))) -∗
+    WP (Exp.allocN (.val (.lit (.int 1))) (.val v)) @ m; M {{ Φ }} := by
+  iintro %Hmask HΦ
+  iapply wp_allocN 1 _ _ (by omega) Hmask
+  iapply m.map $$ HΦ
+  iintro HΦ %l Hpts; ispecialize HΦ $$ %l
+  iapply HΦ; simp [List.range_one, LawfulLoc.add_zero]
+  icases Hpts with ⟨H, -⟩; iframe
+
+theorem wp_load {M : CoPset} (l : Loc) (v : Val) (dq : DFrac) (Φ : Val → IProp GF) :
+    ↑(heapH_inv_name (GF := GF) (Loc := Loc) (Val := Val)) ⊆ M →
+    l ↦{dq} v -∗
+    m iprop(l ↦{dq} v -∗ Φ v) -∗
+    WP (Exp.load (Exp.val (Val.lit (BaseLit.loc l)))) @ m ; M {{ Φ }} := by
+  iintro %Hmask Hpt HΦ
+  simp only [wp_unfold, Exp.denote.eq_16, Exp.isVal, ↓reduceIte]
+  iapply wpi_bind; iapply wp_val
+  iapply wpi_bind; simp only [Val.loc!]
+  iapply wpi_pure; iapply wpi_bind
+  iapply wpi_load! _ _ _ _ _ Hmask $$ Hpt
+  iintro Hpt; iapply wpi_step_pure
+  iapply m.wand $$ HΦ Hpt
+
+theorem wp_store {M : CoPset} (l : Loc) (v v' : Val) (Φ : Val → IProp GF) :
+    ↑(heapH_inv_name (GF := GF) (Loc := Loc) (Val := Val)) ⊆ M →
+    l ↦ v -∗
+    m iprop(l ↦ v' -∗ Φ (.lit .unit)) -∗
+    WP (Exp.store (Exp.val (Val.lit (BaseLit.loc l))) (Exp.val v')) @ m ; M {{ Φ }} := by
+  iintro %Hmask Hpt HΦ
+  simp only [wp_unfold, Exp.denote.eq_17, Exp.isVal, ↓reduceIte]
+  iapply wpi_bind; iapply wp_val
+  iapply wpi_bind; iapply wp_val
+  iapply wpi_bind; simp only [Val.loc!]
+  iapply wpi_pure; iapply wpi_bind
+  iapply wpi_store! _ _ _ _ _ Hmask $$ Hpt
+  iintro Hpt; iapply wpi_step_pure
+  iapply m.wand $$ HΦ Hpt
+
+theorem wp_free {M : CoPset} (l : Loc) (v : Val) (Φ : Val → IProp GF) :
+    ↑(heapH_inv_name (GF := GF) (Loc := Loc) (Val := Val)) ⊆ M →
+    l ↦ v -∗
+    m iprop(l ↦? (none : Option Val) -∗ Φ (.lit .unit)) -∗
+    WP (Exp.free (Exp.val (Val.lit (BaseLit.loc l)))) @ m ; M {{ Φ }} := by
+  iintro %Hmask Hpt HΦ
+  simp only [wp_unfold, Exp.denote.eq_15, Exp.isVal, ↓reduceIte]
+  iapply wpi_bind; iapply wp_val
+  iapply wpi_bind; simp only [Val.loc!]
+  iapply wpi_pure; iapply wpi_bind
+  iapply wpi_storeOpt _ _ _ _ _ Hmask $$ Hpt
+  iintro Hpt; iapply wpi_step_pure
+  iapply m.wand $$ HΦ Hpt
+
+theorem wp_xchg {M : CoPset} (l : Loc) (v v' : Val) (Φ : Val → IProp GF) :
+    ↑(heapH_inv_name (GF := GF) (Loc := Loc) (Val := Val)) ⊆ M →
+    l ↦ v -∗
+    m iprop(l ↦ v' -∗ Φ v) -∗
+    WP (Exp.xchg (Exp.val (Val.lit (BaseLit.loc l))) (Exp.val v')) @ m ; M {{ Φ }} := by
+  iintro %Hmask Hpt HΦ
+  simp only [wp_unfold, Exp.denote.eq_19, Exp.isVal, ↓reduceIte]
+  iapply wpi_bind; iapply wp_val
+  iapply wpi_bind; iapply wp_val
+  iapply wpi_bind; simp only [Val.loc!]
+  iapply wpi_pure; iapply wpi_bind
+  iapply wpi_store! _ _ _ _ _ Hmask $$ Hpt
+  iintro Hpt; iapply wpi_step_pure
+  iapply m.wand $$ HΦ Hpt
+
+theorem wp_cmpXchg_fail {M : CoPset} (l : Loc) (dq : DFrac) (v' v₁ v₂ : Val) (Φ : Val → IProp GF) :
+    ↑(heapH_inv_name (GF := GF) (Loc := Loc) (Val := Val)) ⊆ M →
+    v' ≠ v₁ →
+    v'.compareSafe v₁ = true →
+    l ↦{dq} v' -∗
+    m iprop(l ↦{dq} v' -∗ Φ (.pair v' (.lit (.bool false)))) -∗
+    WP (Exp.cmpXchg (Exp.val $ Val.lit $ BaseLit.loc l) (Exp.val v₁) (Exp.val v₂))
+      @ m ; M {{ Φ }} := by
+  iintro %Hmask %Hneq %Hcmp Hpt HΦ
+  simp only [wp_unfold, Exp.denote.eq_18, Exp.isVal, ↓reduceIte]
+  iapply wpi_bind; iapply wp_val
+  iapply wpi_bind; iapply wp_val
+  iapply wpi_bind; simp only [Val.loc!]; iapply wp_val
+  iapply wpi_bind; simp only
+  iapply wpi_pure; iapply wpi_bind
+  iapply wpi_load! _ _ _ _ _ Hmask $$ Hpt
+  simp only [Hcmp, Hneq, Bool.not_true, Bool.false_eq_true, ↓reduceIte]
+  iintro Hpt; iapply wpi_step_pure
+  iapply m.wand $$ HΦ Hpt
+
+theorem wp_cmpXchg_suc {M : CoPset} (l : Loc) (v' v₁ v₂ : Val) (Φ : Val → IProp GF) :
+    ↑(heapH_inv_name (GF := GF) (Loc := Loc) (Val := Val)) ⊆ M →
+    v' = v₁ →
+    v'.compareSafe v₁ = true →
+    l ↦ v' -∗
+    m iprop(l ↦ v₂ -∗ Φ (.pair v' (.lit $ .bool true))) -∗
+    WP (Exp.cmpXchg (Exp.val $ Val.lit $ BaseLit.loc l) (Exp.val v₁) (Exp.val v₂))
+      @ m ; M {{ Φ }} := by
+  iintro %Hmask %Heq %Hcmp Hpt HΦ; subst Heq
+  simp only [wp_unfold, Exp.denote.eq_18, Exp.isVal, ↓reduceIte]
+  iapply wpi_bind; iapply wp_val
+  iapply wpi_bind; iapply wp_val
+  iapply wpi_bind; iapply wp_val
+  iapply wpi_bind; simp only [Val.loc!]
+  iapply wpi_pure; iapply wpi_bind
+  iapply wpi_load! _ _ _ _ _ Hmask $$ Hpt
+  simp only [Hcmp, Bool.not_true, Bool.false_eq_true, ↓reduceIte]
+  iintro Hpt; iapply wpi_bind
+  iapply wpi_store! _ _ _ _ _ Hmask $$ Hpt
+  iintro Hpt; iapply wpi_step_pure
+  iapply m.wand $$ HΦ Hpt
+
+theorem wp_faa {M : CoPset} (l : Loc) (i₁ i₂ : Int) (Φ : Val → IProp GF) :
+    ↑(heapH_inv_name (GF := GF) (Loc := Loc) (Val := Val)) ⊆ M →
+    l ↦ Val.lit (.int i₁) -∗
+    m iprop(l ↦ (.lit (.int (i₁ + i₂)) : Val) -∗ Φ (.lit (.int i₁))) -∗
+    WP (Exp.faa (.val $ .lit $ .loc l) (.val $ .lit $ .int i₂)) @ m ; M {{ Φ }} := by
+  iintro %Hmask Hpt HΦ
+  simp only [wp_unfold, Exp.denote.eq_20, Exp.isVal, ↓reduceIte]
+  iapply wpi_bind; iapply wp_val
+  iapply wpi_bind; iapply wp_val
+  iapply wpi_bind; simp only [Val.loc!]
+  iapply wpi_pure; iapply wpi_bind; simp only [Val.int!]
+  iapply wpi_pure; iapply wpi_bind
+  iapply wpi_load! _ _ _ _ _ Hmask $$ Hpt; simp only
+  iintro Hpt; iapply wpi_bind; iapply wpi_pure; iapply wpi_bind
+  iapply wpi_store! _ _ _ _ _ Hmask $$ Hpt
+  iintro Hpt; iapply wpi_step_pure
+  iapply m.wand $$ HΦ Hpt
+
+end heap_rules
+
+end wp_rules
